test_proof.lean
@@ -1,3 +1,0 @@
-import Blanc.NewCommon
-lemma test (x : UInt8) : (x.highs <<< 4) ||| x.lows = x := by
-  decide
